working on automation

start.v
@@ -5,6 +5,9 @@ From Coq Require Import Arith.Arith.
 From Coq Require Import Arith.EqNat. Import Nat.
 From Coq Require Import Strings.String.
 
+Open Scope list.
+Open Scope string.
+
 (* locations are strings *)
 Definition location := string.
 Definition lifetime := string.
@@ -59,6 +62,10 @@ Inductive partial_type :=
   | PYUndefined.
 
 
+Coercion VInt : nat >-> value.
+Coercion LVar : string >-> lval.
+Notation "'#' v" := (PVDefined v) (at level 0).
+Notation "'##'" := (PVUndefined) (at level 0).
 
 (* state *)
 Definition store := list (location * (partial_value * lifetime)).
@@ -71,33 +78,12 @@ Definition s_alloc (st : store) (l : location) (pv_l : partial_value * lifetime)
 Fixpoint s_in (st :store) (l : location) 
   : partial_value * lifetime :=
   match st with
-  | nil => (PVUndefined, "global"%string)
+  | nil => (##, "global")
   | ((cl, pv_l) :: tl)%list => if (eqb cl l) then pv_l else s_in tl l
   end.
 
 
-Compute s_alloc nil "lx"%string (PVDefined VUnit, "l"%string).
-
-(* stuff for maps from Maps.v*)
-(*
-Definition total_map (A : Type) := string -> A.
-
-Definition t_empty {A : Type} (v : A) : total_map A :=
-  (fun _ => v).
-
-Definition t_update {A : Type} (m : total_map A)
-                    (x : string) (v : A) :=
-                    fun x' => if String.eqb x x' then v else m x'.
-
-(* map notation *)
-Notation "'_' '!->' v" := (t_empty v)
-  (at level 100, right associativity).
-
-Notation "x '!->' v ';' m" := (t_update m x v)
-                              (at level 100, v at next level, right associativity).
-
-*)
-
+Compute s_alloc nil "lx" (# VUnit, "l").
 
 (* 
    store : locations -> (partial_value * lifetimes)
@@ -107,12 +93,11 @@ Notation "x '!->' v ';' m" := (t_update m x v)
  *)
 (* Definition store := total_map (partial_value * lifetime). *)
 
-
 Definition example_store := (
-  ("x"%string, (PVDefined (VInt 1),         "l_l"%string)) ::
-  ("p"%string, (PVDefined (VBorrowRef "x"), "l_m"%string)) ::
-  ("d"%string, (PVDefined (VBorrowRef "p"), "l_f"%string)) ::
-  ("t"%string, (PVDefined (VBorrowRef "d"), "l_a"%string)) ::
+  ("x", (#1 ,         "l_l")) ::
+  ("p", (# (VBorrowRef "x"), "l_m")) ::
+  ("d", (# (VBorrowRef "p"), "l_f")) ::
+  ("t", (# (VBorrowRef "d"), "l_a")) ::
     nil
   )%list.
 
@@ -120,73 +105,139 @@ Definition example_store := (
 
 Inductive loc : store -> lval -> location -> Prop :=
   | Loc_Var : forall (st : store) (var_loc : string), 
-      ~ (fst (s_in st var_loc)) = PVUndefined ->
+      ~ (fst (s_in st var_loc)) = ## ->
       loc st (LVar var_loc) var_loc
   | Loc_Deref : 
       forall (st : store) (l lw: location) (w : lval),
       (
-        fst (s_in st lw) = PVDefined (VBorrowRef l) \/
-        fst (s_in st lw) = PVDefined (VOwnRef l)
+        fst (s_in st lw) = # (VBorrowRef l) \/
+        fst (s_in st lw) = # (VOwnRef l)
       ) ->
       loc st w lw ->
       loc st (LDeref w) l.
-
-Example loc_ex1 : loc example_store (LVar "x"%string) "x"%string.
-Proof.
-  apply Loc_Var. simpl. unfold not. intros H. discriminate.
-Qed.
-
-Example loc_ex2 : loc example_store (LVar "p"%string) "t"%string.
-Proof.
-  (* we are stuck because t != p*)
-Abort.
-
-Example loc_ex3 : loc example_store (LVar "y"%string) "y"%string.
-Proof.
-  apply Loc_Var. simpl. 
-  (* we are stuck because there is no y in example_store *)
-Abort.
-
-Example loc_ex4 : loc example_store (LDeref (LVar "p"%string)) "x"%string.
-Proof.
-  apply Loc_Deref with (lw := "p"%string). 
-  + simpl. left. reflexivity.
-  + apply Loc_Var. intros H. simpl in H. discriminate.
-Qed.
 
 Ltac loc_var := apply Loc_Var; unfold not; intros H; discriminate.
 Ltac loc_deref s := apply Loc_Deref with (lw := s); 
   simpl; try (left; reflexivity); try (right; reflexivity); try (loc_var).
 
-Example loc_ex5 : loc example_store (LDeref (LVar "d"%string)) "p"%string.
+Fixpoint find_loc (st : store) (s : string) : string :=
+  match st with
+  | nil => ""
+  | (l,(# (VBorrowRef l'),_)) :: st' => if (l' =? s)%string
+      then l
+      else find_loc st' s
+  | (l,(# (VOwnRef l'),_)) :: st' => if (l' =? s)%string
+      then l
+      else find_loc st' s
+  | _ :: st' => find_loc st' s
+  end.
+
+Fixpoint deref_loc (st : store) (s : string) : string :=
+  match st with
+  | nil => ""
+  | (l,(# (VBorrowRef l'),_)) :: st' => if (l =? s)%string
+      then l'
+      else deref_loc st' s
+  | (l,(# (VOwnRef l'),_)) :: st' => if (l =? s)%string
+      then l'
+      else deref_loc st' s
+  | _ :: st' => deref_loc st' s
+  end.
+
+Fixpoint deref_loc_repeat (st : store) (w : lval) : string :=
+  match w with 
+  | LVar s => s
+  | LDeref o => deref_loc st (deref_loc_repeat st o)
+  end.
+
+
+Ltac auto_loc :=
+  repeat match goal with
+  | [ |- loc ?st (LVar ?x) ?y ] => loc_var
+  | [ |- loc ?st (LDeref (LVar ?l)) ?y ] => loc_deref l
+  | [ |- loc ?st ?a ?y ] => try loc_deref (find_loc st y)
+  end.
+
+
+Example loc_ex1 : loc example_store (LVar "x") "x".
 Proof.
-  loc_deref "d"%string.
+  apply Loc_Var. simpl. unfold not. intros H. discriminate.
 Qed.
 
-Example loc_ex6 : loc example_store (LDeref (LDeref (LVar "d"%string))) "x"%string.
+Example loc_ex1' : loc example_store (LVar "x") "x".
 Proof.
-  apply Loc_Deref with (lw := "p"%string). 
+  auto_loc.
+Qed.
+
+Example loc_ex2 : loc example_store (LVar "p") "t".
+Proof.
+  (* we are stuck because t != p*)
+Abort.
+
+Example loc_ex3 : loc example_store (LVar "y") "y".
+Proof.
+  apply Loc_Var. simpl. 
+  (* we are stuck because there is no y in example_store *)
+Abort.
+
+Example loc_ex4 : loc example_store (LDeref (LVar "p")) "x".
+Proof.
+  apply Loc_Deref with (lw := "p"). 
   + simpl. left. reflexivity.
-  + apply Loc_Deref with (lw := "d"%string).
+  + apply Loc_Var. intros H. simpl in H. discriminate.
+Qed.
+
+Example loc_ex4' : loc example_store (LDeref (LVar "p")) "x".
+Proof.
+  auto_loc.
+Qed.
+
+
+Example loc_ex5 : loc example_store (LDeref (LVar "d")) "p".
+Proof.
+  auto_loc.
+Qed.
+
+Example loc_ex6 : loc example_store (LDeref (LDeref (LVar "d"))) "x".
+Proof.
+  apply Loc_Deref with (lw := "p"). 
+  + simpl. left. reflexivity.
+  + apply Loc_Deref with (lw := "d").
     - simpl. left. reflexivity.
     - apply Loc_Var. intros H. discriminate.
 Qed.
 
-Example loc_ex6' : loc example_store (LDeref (LDeref (LVar "d"%string))) "x"%string.
+Example loc_ex6' : loc example_store (LDeref (LDeref (LVar "d"))) "x".
 Proof.
-  loc_deref "p"%string. loc_deref "d"%string.
+  loc_deref "p". loc_deref "d".
+Qed.
+
+Example loc_ex6'' : loc example_store (LDeref (LDeref (LVar "d"))) "x".
+Proof.
+  auto_loc.
 Qed.
 
 Example loc_ex7 : 
-  loc example_store (LDeref (LDeref (LDeref (LVar "t"%string)))) "x"%string.
+  loc example_store (LDeref (LDeref (LDeref (LVar "t")))) "x".
 Proof.
-  loc_deref "p"%string. loc_deref "d"%string. loc_deref "t"%string.
+  loc_deref "p". loc_deref "d". loc_deref "t".
+Qed.
+
+Example loc_ex7' : 
+  loc example_store (LDeref (LDeref (LDeref (LVar "t")))) "x".
+Proof.
+  auto_loc.
 Qed.
 
 Example loc_ex8 : 
-  loc example_store (LDeref (LVar "x"%string)) "x"%string.
+  loc example_store (LDeref (LVar "x")) "x".
 Proof.
-loc_deref "x"%string. Abort. (* we are stuck because x is not a ref*)
+loc_deref "x". Abort. (* we are stuck because x is not a ref*)
+
+Example loc_ex8 : 
+  loc example_store (LDeref (LVar "x")) "x".
+Proof.
+auto_loc. Abort. (* we are stuck because x is not a ref*)
 
 Inductive read: store -> lval -> partial_value * lifetime -> Prop :=
   | Read : forall (st : store) (w : lval) (pv_l : partial_value * lifetime) (l : location), 
@@ -194,42 +245,78 @@ Inductive read: store -> lval -> partial_value * lifetime -> Prop :=
       loc st w l ->
       read st w pv_l.
 
+Ltac read_rule s :=
+      apply Read with (l := s);
+      try (simpl; reflexivity); try auto_loc.
+
+Ltac auto_read :=
+  match goal with 
+  | [ |- read ?st (LVar ?l) ?pv ] => read_rule l
+  | [ |- read ?st ?d ?pv ] => read_rule (deref_loc_repeat st d)
+  end.
+
 Example read_ex1 :
-  read example_store (LVar "x"%string) ((PVDefined (VInt 1)), "l_l"%string).
+  read example_store (LVar "x") (#1, "l_l").
 Proof.
-  apply Read with (l := "x"%string). 
+  apply Read with (l := "x"). 
   + simpl. reflexivity.
   + loc_var.
+Qed.
+
+Example read_ex1' :
+  read example_store (LVar "x") (#1, "l_l").
+Proof.
+  auto_read.
 Qed.
 
 Example read_ex2 :
-  read example_store (LVar "p"%string) ((PVDefined (VBorrowRef "x"%string)), "l_m"%string).
+  read example_store (LVar "p") (#(VBorrowRef "x"), "l_m").
 Proof.
-  apply Read with (l := "p"%string). 
+  apply Read with (l := "p"). 
   + simpl. reflexivity.
   + loc_var.
 Qed.
 
-Example read_ex3 :
-  read example_store (LDeref (LVar "p"%string)) ((PVDefined (VInt 1)), "l_l"%string).
+Example read_ex2' :
+  read example_store (LVar "p") (#(VBorrowRef "x"), "l_m").
 Proof.
-  apply Read with (l := "x"%string).
+  auto_read.
+Qed.
+
+Example read_ex3 :
+  read example_store (LDeref (LVar "p")) ((#1), "l_l").
+Proof.
+  apply Read with (l := "x").
   + simpl. reflexivity.
-  + loc_deref "p"%string.
+  + loc_deref "p".
+Qed.
+
+Example read_ex3' :
+  read example_store (LDeref (LVar "p")) ((#1), "l_l"). 
+Proof.
+  auto_read.
 Qed.
 
 Example read_ex4 :
-  read example_store (LDeref (LDeref (LVar "d"%string))) ((PVDefined (VInt 1)), "l_l"%string).
+  read example_store (LDeref (LDeref (LVar "d"))) ((#1), "l_l").
 Proof.
-  apply Read with (l := "x"%string).
+  apply Read with (l := "x").
   + simpl. reflexivity.
-  + loc_deref "p"%string. loc_deref "d"%string.
+  + loc_deref "p". loc_deref "d".
 Qed.
 
+Example read_ex4' :
+  read example_store (LDeref (LDeref (LVar "d"))) ((#1), "l_l").
+Proof.
+  auto_read.
+Qed.
+
+
+
 Example read_ex5 :
-  read nil (LVar "x"%string) (PVUndefined, "global"%string).
+  read nil "x" (##, "global").
 Proof. 
-  apply Read with (l := "x"%string).
+  apply Read with (l := "x").
   + simpl. reflexivity.
   + apply Loc_Var. intros H.
   simpl in H. Abort .
@@ -248,28 +335,28 @@ Inductive write: store -> lval -> partial_value -> store -> Prop :=
 
 
 Definition es_1 :=
-  ( ("x"%string, (PVDefined (VInt 0),         "lifetime_l"%string)) ::
+  ( ("x", (#0,         "lifetime_l")) ::
     nil
   )%list.
 
 Definition es_1' :=
-  ( ("x"%string, (PVDefined (VInt 1),         "lifetime_l"%string)) ::
+  ( ("x", (#1,         "lifetime_l")) ::
     nil
   )%list.
 
 Example write_ex1 :
-  write nil (LVar "x"%string) (PVDefined (VInt 0)) es_1.
+  write nil (LVar "x") (#0) es_1.
 Proof.
-  apply Write with (l := "x"%string).
+  apply Write with (l := "x").
   + simpl. reflexivity.
   + apply Loc_Var. intros H. simpl in H. 
   Abort.
     (* this fails because x was not defined in st*)
 
 Example write_ex2 :
-  write es_1 (LVar "x"%string) (PVDefined (VInt 1)) es_1'.
+  write es_1 (LVar "x") (#1) es_1'.
 Proof.
-  apply Write with (l := "x"%string).
+  apply Write with (l := "x").
   - simpl. reflexivity.
   - loc_var.
   Qed.
@@ -277,23 +364,23 @@ Proof.
 
 Definition es_2 :=
   ( 
-  ("x"%string, (PVDefined (VInt 1),         "lifetime_l"%string)) ::
-  ("p"%string, (PVDefined (VBorrowRef "x"), "lifetime_g"%string)) ::
+  ("x", (#1,         "lifetime_l")) ::
+  ("p", (# (VBorrowRef "x"), "lifetime_g")) ::
   nil
   )%list.
 Definition es_3 :=
   ( 
-  ("x"%string, (PVDefined (VInt 2),         "lifetime_l"%string)) ::
-  ("p"%string, (PVDefined (VBorrowRef "x"), "lifetime_g"%string)) ::
+  ("x", (#2,         "lifetime_l")) ::
+  ("p", (# (VBorrowRef "x"), "lifetime_g")) ::
   nil
   )%list.
 
 Example write_ex3 :
-  write es_2 (LDeref (LVar "p"%string)) (PVDefined (VInt 2)) es_3.
+  write es_2 (LDeref (LVar "p")) (#2) es_3.
 Proof.
-  apply Write with (l := "x"%string).
+  apply Write with (l := "x").
   + simpl. reflexivity.
-  + loc_deref "p"%string.
+  + loc_deref "p".
 Qed.
 
 
@@ -304,7 +391,7 @@ Qed.
 Fixpoint remove_location (st : store) (l : location) : store :=
   match st with
   | nil => nil
-  | (hd :: tl)%list => if (eqb l (fst hd))%string 
+  | (hd :: tl)%list => if (eqb l (fst hd)) 
       then remove_location tl l 
       else (hd :: remove_location tl l)%list
   end.
@@ -319,7 +406,7 @@ Fixpoint collect_in_scope (st : store) (lf : lifetime) (lst : list location)
   : list location :=
   match st with 
   | nil => lst
-  | ((l, (pv, clf)) :: tl)%list => if (eqb clf lf)%string
+  | ((l, (pv, clf)) :: tl)%list => if (eqb clf lf)
       then collect_in_scope tl lf (l :: lst)%list
       else collect_in_scope tl lf lst
   end.
@@ -335,32 +422,32 @@ Inductive drop : store -> list partial_value -> store -> Prop :=
   | D_nil : forall (st : store),
       drop st nil st
   | D_cons_other : forall (st : store) (pv : partial_value) (tl : list partial_value),
-      (forall (l : location), (pv <> PVDefined (VOwnRef l))) ->
+      (forall (l : location), (pv <> # (VOwnRef l))) ->
       drop st (cons pv tl) st
   | D_cons_own : forall (st1 st2 st3 : store)
       (tl : list partial_value) (l l_own : location),
-      fst (s_in st1 l_own) = (PVDefined (VOwnRef l)) ->
+      fst (s_in st1 l_own) = (# (VOwnRef l)) ->
       st2 = remove_location st1 l_own ->
       drop st2 (cons (fst (s_in st1 l)) tl) st3  ->
-      drop st1 (cons (PVDefined (VOwnRef l)) tl) st2.
+      drop st1 (cons (# (VOwnRef l)) tl) st2.
 
 Definition drop_ex1_st1 : store :=
   (
-    ("lx"%string, ((PVDefined (VInt 1)),"l"%string)) ::
-    ("lp"%string, ((PVDefined (VOwnRef "lx"%string)),"m"%string)) ::
+    ("lx", ((#1),"l")) ::
+    ("lp", ((# (VOwnRef "lx")),"m")) ::
     nil
   )%list.
 
 Definition drop_ex1_st2 : store :=
   (
-    ("lx"%string, ((PVDefined (VInt 1)),"l"%string)) ::
+    ("lx", ((#1),"l")) ::
     nil
   )%list.
 
 Example drop_ex1 : drop drop_ex1_st1 
-  (collect_pvs drop_ex1_st1 ("lp"%string :: nil)%list nil) 
+  (collect_pvs drop_ex1_st1 ("lp" :: nil)%list nil) 
   drop_ex1_st2.
-Proof. simpl. apply D_cons_own with (st3 := drop_ex1_st2) (l_own := "lp"%string).
+Proof. simpl. apply D_cons_own with (st3 := drop_ex1_st2) (l_own := "lp").
 + reflexivity.
 + reflexivity.
 + simpl. apply D_cons_other. unfold not. intros l H. injection H as H1. discriminate.
@@ -371,15 +458,15 @@ Reserved Notation " t '-->' t' '|' l " (at level 40).
 
 Inductive step : lifetime -> (term * store) -> (term * store) -> Prop :=
 | R_Copy : forall (w : lval) (v : value) (lf slf : lifetime) (st : store),
-    read st w (PVDefined v, lf) ->
+    read st w (# v, lf) ->
     (TCopy w, st) --> (TValue v, st) | slf
 | R_Move : forall (w : lval) (v : value) (lf slf : lifetime) (st1 st2 : store),
-    read st1 w (PVDefined v, lf) ->
-    write st1 w PVUndefined st2 ->
+    read st1 w (# v, lf) ->
+    write st1 w ## st2 ->
     (TMove w, st1) --> (TValue v, st2) | slf
 | R_Box : forall (v : value) (n : location) (slf : lifetime) (st1 st2 : store),
-    fst (s_in st1 n) = PVUndefined ->
-    st2 = cons (n, (PVDefined v, "global"%string)) st1 ->
+    fst (s_in st1 n) = ## ->
+    st2 = cons (n, (# v, "global")) st1 ->
     (THeapAlloc (TValue v), st1) --> (TValue (VOwnRef n), st2) | slf
 | R_Borrow : forall (w : lval) (lw : location) (slf : lifetime) (st : store),
     loc st w lw ->
@@ -391,13 +478,13 @@ Inductive step : lifetime -> (term * store) -> (term * store) -> Prop :=
     (w : lval) (v2 : value) (pv1 : partial_value * lifetime) (slf : lifetime),
     read st1 w pv1 ->
     drop st1 (fst pv1 :: nil)%list st2 ->
-    write st2 w (PVDefined v2) st3 ->
+    write st2 w (# v2) st3 ->
     (TAssignment w (TValue v2), st1) --> (TValue VUnit, st3) | slf
 | R_Declare : forall (v : value) (lx : location) (x : string) (slf : lifetime) (st1 st2 : store),
-    st2 = cons (lx, (PVDefined v, slf)) st1 ->
+    st2 = cons (lx, (# v, slf)) st1 ->
     (TDeclaration x (TValue v), st1) --> (TValue VUnit, st2) | slf
 | R_Seq : forall (st1 st2 : store) (v : value) (t : term) (slf : lifetime),
-    drop st1 (PVDefined v :: nil)%list st2 ->
+    drop st1 (# v :: nil)%list st2 ->
     (TSeq (TValue v) t, st1) --> (t, st2) | slf
 | R_BlockA : forall (st1 st2 : store) (l_lf m_lf : lifetime) (t1 t2 : term),
     (t1, st1) --> (t2, st2) | m_lf ->
@@ -410,33 +497,54 @@ Inductive step : lifetime -> (term * store) -> (term * store) -> Prop :=
     (THeapAlloc t1, st1) --> (THeapAlloc t2, st2) | l_lf
 | R_Sub_Seq : forall (st1 st2 : store) (l_lf : lifetime) (t1 t2 t3 : term),
     (t1,st1) --> (t2,st2) | l_lf ->
-    (TSeq t1 t2, st1) --> (t3, st2) | l_lf
+    (TSeq t1 t3, st1) --> (TSeq t2 t3, st2) | l_lf
+| R_Sub_Asg : forall (st1 st2 : store) (l_lf : lifetime) (t1 t2 : term) (w : lval),
+    (t1,st1) --> (t2,st2) | l_lf ->
+    (TAssignment w t1, st1) --> (TAssignment w t2, st2) | l_lf
+| R_Sub_Decl : forall (st1 st2 : store) (l_lf : lifetime) (t1 t2 : term) (x : string),
+    (t1,st1) --> (t2,st2) | l_lf ->
+    (TDeclaration x t1, st1) --> (TDeclaration x t2, st2) | l_lf
 where " t '-->' t' '|' l " := (step l t t').
 
-(* figuring out R_Sub *)
-Open Scope list.
-Open Scope string.
+Check step.
 
-Definition r_sub1_st := ("y", (PVDefined (VInt 1), "l_lf")) :: nil.
-Example r_sub1: (THeapAlloc (TCopy (LVar "y")),r_sub1_st) --> 
-  (THeapAlloc (TValue (VInt 1)) ,r_sub1_st) | "l_lf".
+Inductive multi : Prop -> Prop :=
+  | multi_refl : forall (ts : term * store) (lf : lifetime),
+      multi (ts --> ts | lf)
+  | multi_step : forall (ts1 ts2 ts3 : term * store) (lf : lifetime),
+      (ts1 --> ts2 | lf) ->
+      multi (ts2 --> ts3 | lf) ->
+      multi (ts1 --> ts3 | lf).
+
+Notation " t '-->*' t' | lf" := (multi (t --> t' | lf)) (at level 40).
+
+(* figuring out R_Sub *)
+
+Definition r_sub1_st := ("y", (#1, "l_lf")) :: nil.
+Example r_sub1: (THeapAlloc (TCopy (LVar "y")),r_sub1_st) -->
+  (THeapAlloc (TValue 1) ,r_sub1_st) | "l_lf".
 Proof.
-  apply R_Sub_HeapAlloc.
-  apply R_Copy with (lf := "l_lf").
-  + apply Read with (l := "y").
-    - reflexivity.
-    - loc_var.
+    apply R_Sub_HeapAlloc.
+    apply R_Copy with (lf := "l_lf").
+      + apply Read with (l := "y").
+    reflexivity.
+    loc_var.
 Qed.
 
-Definition r_sub2_st  := ("y", (PVDefined (VInt 1), "l_lf")) :: nil.
-Definition r_sub2_st' := ("y", (PVDefined (VInt 2), "l_lf")) :: nil.
+Definition r_sub2_st  := ("y", (#1, "l_lf")) :: nil.
+Definition r_sub2_st' := ("y", (#2, "l_lf")) :: nil.
 Example r_sub2: 
-  (TSeq (TAssignment (LVar "y") (TValue (VInt 2))) (TValue VUnit)
+  (TSeq 
+    (TAssignment (LVar "y") (TValue 2)) 
+    (TAssignment (LVar "x") (TMove (LVar "y")))
   ,r_sub2_st) 
   --> 
-  (TSeq (TValue VUnit) (TValue VUnit) ,r_sub2_st') | "l_lf".
+  (TSeq 
+    (TValue VUnit) 
+    (TAssignment (LVar "x") (TMove (LVar "y")))
+  ,r_sub2_st') | "l_lf".
 Proof.
-  apply R_Sub_Seq. apply R_Assign with (st2 := r_sub2_st) (pv1 := (PVDefined (VInt 1), "l_lf")).
+  apply R_Sub_Seq. apply R_Assign with (st2 := r_sub2_st) (pv1 := (#1, "l_lf")).
   + apply Read with (l := "y").
     - simpl. reflexivity.
     - loc_var.
@@ -448,49 +556,23 @@ Proof.
 
 (* worked example 1 *)
 
-Definition we1_0 : (term * store) :=
-  (
-  TBlock (
-  TSeq 
-    (TDeclaration "x"%string (TValue (VInt 1)))
-    (
-    TSeq
-      (TDeclaration "y"%string (THeapAlloc (TCopy (LVar "x"%string))))
-      (TBlock (
-      TSeq 
-        (TDeclaration "z"%string (THeapAlloc (TValue (VInt 0))))
-        (
-        TSeq
-          (TAssignment (LVar "y"%string) (TBorrow (LVar "z"%string)))
-          (
-          TSeq
-            (TAssignment (LVar "y"%string) (TMove (LVar "z"%string)))
-            (
-            TSeq
-              (TMove (LDeref (LVar "y")))
-              (TValue VUnit)
-            )
-          )
-        )
-      ) "m_lf"%string)
-    )
-  ) "l_lf"%string
-  ,
-  nil
-  ).
-
 Definition we1_1 : (term * store) :=
   (
   TBlock (
+  TSeq 
+    (TDeclaration "x" (TValue 1))
+    (
+    TSeq
+      (TDeclaration "y" (THeapAlloc (TCopy (LVar "x"))))
       (TBlock (
       TSeq 
-        (TDeclaration "z"%string (THeapAlloc (TValue (VInt 0))))
+        (TDeclaration "z" (THeapAlloc (TValue 0)))
         (
         TSeq
-          (TAssignment (LVar "y"%string) (TBorrow (LVar "z"%string)))
+          (TAssignment (LVar "y") (TBorrow (LVar "z")))
           (
           TSeq
-            (TAssignment (LVar "y"%string) (TMove (LVar "z"%string)))
+            (TAssignment (LVar "y") (TMove (LVar "z")))
             (
             TSeq
               (TMove (LDeref (LVar "y")))
@@ -498,18 +580,482 @@ Definition we1_1 : (term * store) :=
             )
           )
         )
-      ) "m_lf"%string)
-  ) "l_lf"%string
+      ) "m_lf")
+    )
+  ) "l_lf"
   ,
-  (
-  ("lx"%string, (PVDefined (VInt 1), "l_lf"%string)) ::
-  ("ly"%string, (PVDefined (VOwnRef "l1"%string), "l_lf"%string)) ::
-  ("l1"%string, (PVDefined (VInt 1), "global"%string)) ::
   nil
-  )%list
   ).
 
-Example we1_step_0_1 : we1_0 --> we1_1 | "l_lf"%string.
+Definition we1_1_1 : (term * store) :=
+  (
+  TBlock (
+  TSeq 
+    (TValue VUnit)
+    (
+    TSeq
+      (TDeclaration "y" (THeapAlloc (TCopy (LVar "x"))))
+      (TBlock (
+      TSeq 
+        (TDeclaration "z" (THeapAlloc (TValue 0)))
+        (
+        TSeq
+          (TAssignment (LVar "y") (TBorrow (LVar "z")))
+          (
+          TSeq
+            (TAssignment (LVar "y") (TMove (LVar "z")))
+            (
+            TSeq
+              (TMove (LDeref (LVar "y")))
+              (TValue VUnit)
+            )
+          )
+        )
+      ) "m_lf")
+    )
+  ) "l_lf"
+  ,
+  ("x", (#1, "l_lf"))
+  :: nil
+  ).
+
+Example we1_step1_1 : we1_1 --> we1_1_1 | "l_lf".
+Proof.
+  apply R_BlockA. apply R_Sub_Seq.
+  - apply R_Declare with (lx := "x").
+    reflexivity.
+Qed.
+
+Definition we1_1_2 : (term * store) :=
+  (
+  TBlock (
+    TSeq
+      (TDeclaration "y" (THeapAlloc (TCopy (LVar "x"))))
+      (TBlock (
+      TSeq 
+        (TDeclaration "z" (THeapAlloc (TValue 0)))
+        (
+        TSeq
+          (TAssignment (LVar "y") (TBorrow (LVar "z")))
+          (
+          TSeq
+            (TAssignment (LVar "y") (TMove (LVar "z")))
+            (
+            TSeq
+              (TMove (LDeref (LVar "y")))
+              (TValue VUnit)
+            )
+          )
+        )
+      ) "m_lf")
+  ) "l_lf"
+  ,
+  ("x", (#1, "l_lf"))
+  :: nil
+  ).
+
+Example we1_step1_2 : we1_1_1 --> we1_1_2 | "l_lf".
 Proof.
   apply R_BlockA.
+  apply R_Seq.
+  apply D_cons_other.
+  intros l. intros H.
+  discriminate.
+Qed.
 
+Definition we1_1_3 : (term * store) :=
+  (
+  TBlock (
+    TSeq
+      (TDeclaration "y" (THeapAlloc (TValue 1)))
+      (TBlock (
+      TSeq 
+        (TDeclaration "z" (THeapAlloc (TValue 0)))
+        (
+        TSeq
+          (TAssignment (LVar "y") (TBorrow (LVar "z")))
+          (
+          TSeq
+            (TAssignment (LVar "y") (TMove (LVar "z")))
+            (
+            TSeq
+              (TMove (LDeref (LVar "y")))
+              (TValue VUnit)
+            )
+          )
+        )
+      ) "m_lf")
+  ) "l_lf"
+  ,
+  ("x", (#1, "l_lf"))
+  :: nil
+  ).
+
+Example we1_step1_3 : we1_1_2 --> we1_1_3 | "l_lf".
+Proof.
+  apply R_BlockA.
+  apply R_Sub_Seq.
+  apply R_Sub_Decl.
+  apply R_Sub_HeapAlloc.
+  apply R_Copy with (lf := "l_lf").
+  apply Read with (l := "x").
+  - simpl. reflexivity.
+  - loc_var.
+Qed.
+
+Definition we1_1_4 : (term * store) :=
+  (
+  TBlock (
+    TSeq
+      (TDeclaration "y" (TValue (VOwnRef "1")))
+      (TBlock (
+      TSeq 
+        (TDeclaration "z" (THeapAlloc (TValue 0)))
+        (
+        TSeq
+          (TAssignment (LVar "y") (TBorrow (LVar "z")))
+          (
+          TSeq
+            (TAssignment (LVar "y") (TMove (LVar "z")))
+            (
+            TSeq
+              (TMove (LDeref (LVar "y")))
+              (TValue VUnit)
+            )
+          )
+        )
+      ) "m_lf")
+  ) "l_lf"
+  ,
+  ("1", (#1, "global")) ::
+  ("x", (#1, "l_lf"))
+  :: nil
+  ).
+
+Example we1_step1_4 : we1_1_3 --> we1_1_4 | "l_lf".
+Proof.
+  apply R_BlockA.
+  apply R_Sub_Seq.
+  apply R_Sub_Decl.
+  apply R_Box.
+  - auto.
+  - auto.
+Qed.
+
+Definition we1_1_5 : (term * store) :=
+  (
+  TBlock (
+    TSeq
+      (TValue VUnit)
+      (TBlock (
+      TSeq 
+        (TDeclaration "z" (THeapAlloc (TValue 0)))
+        (
+        TSeq
+          (TAssignment (LVar "y") (TBorrow (LVar "z")))
+          (
+          TSeq
+            (TAssignment (LVar "y") (TMove (LVar "z")))
+            (
+            TSeq
+              (TMove (LDeref (LVar "y")))
+              (TValue VUnit)
+            )
+          )
+        )
+      ) "m_lf")
+  ) "l_lf"
+  ,
+  ("y", (# (VOwnRef "1"), "l_lf")) ::
+  ("1", (#1, "global")) ::
+  ("x", (#1, "l_lf"))
+  :: nil
+  ).
+
+Example we1_step1_5 : we1_1_4 --> we1_1_5 | "l_lf".
+Proof.
+  apply R_BlockA.
+  apply R_Sub_Seq.
+  apply R_Declare with (lx := "y").
+  auto.
+Qed.
+
+Definition we1_2 : (term * store) :=
+  (
+  TBlock (
+      (TBlock (
+      TSeq 
+        (TDeclaration "z" (THeapAlloc (TValue 0)))
+        (
+        TSeq
+          (TAssignment (LVar "y") (TBorrow (LVar "z")))
+          (
+          TSeq
+            (TAssignment (LVar "y") (TMove (LVar "z")))
+            (
+            TSeq
+              (TMove (LDeref (LVar "y")))
+              (TValue VUnit)
+            )
+          )
+        )
+      ) "m_lf")
+  ) "l_lf"
+  ,
+  ("y", (# (VOwnRef "1"), "l_lf")) ::
+  ("1", (#1, "global")) ::
+  ("x", (#1, "l_lf"))
+  :: nil
+  ).
+
+Example we1_step1_6 : we1_1_5 --> we1_2 | "l_lf".
+Proof.
+  apply R_BlockA.
+  apply R_Seq.
+  apply D_cons_other.
+  intros l H.
+  discriminate.
+Qed.
+
+Example we1_step1 : we1_1 -->* we1_2 | "l_lf".
+Proof.
+  apply multi_step with (ts2 := we1_1_1); try (apply we1_step1_1).
+  apply multi_step with (ts2 := we1_1_2); try (apply we1_step1_2).
+  apply multi_step with (ts2 := we1_1_3); try (apply we1_step1_3).
+  apply multi_step with (ts2 := we1_1_4); try (apply we1_step1_4).
+  apply multi_step with (ts2 := we1_1_5); try (apply we1_step1_5).
+  apply multi_step with (ts2 := we1_2); try (apply we1_step1_6).
+  apply multi_refl.
+Qed.
+
+Definition we1_2_1 : (term * store) :=
+  (
+  TBlock (
+      (TBlock (
+      TSeq 
+        (TDeclaration "z" (TValue (VOwnRef "2")))
+        (
+        TSeq
+          (TAssignment (LVar "y") (TBorrow (LVar "z")))
+          (
+          TSeq
+            (TAssignment (LVar "y") (TMove (LVar "z")))
+            (
+            TSeq
+              (TMove (LDeref (LVar "y")))
+              (TValue VUnit)
+            )
+          )
+        )
+      ) "m_lf")
+  ) "l_lf"
+  ,
+  ("2", (#0, "global")) ::
+  ("y", (# (VOwnRef "1"), "l_lf")) ::
+  ("1", (#1, "global")) ::
+  ("x", (#1, "l_lf"))
+  :: nil
+  ).
+
+Example we1_step2_1 : we1_2 --> we1_2_1 | "l_lf".
+Proof.
+  apply R_BlockA.
+  apply R_BlockA.
+  apply R_Sub_Seq.
+  apply R_Sub_Decl.
+  apply R_Box with (n := "2").
+  - auto.
+  - auto.
+Qed.
+
+Definition we1_2_2 : (term * store) :=
+  (
+  TBlock (
+      (TBlock (
+      TSeq 
+        (TValue VUnit)
+        (
+        TSeq
+          (TAssignment (LVar "y") (TBorrow (LVar "z")))
+          (
+          TSeq
+            (TAssignment (LVar "y") (TMove (LVar "z")))
+            (
+            TSeq
+              (TMove (LDeref (LVar "y")))
+              (TValue VUnit)
+            )
+          )
+        )
+      ) "m_lf")
+  ) "l_lf"
+  ,
+  ("z", (# (VOwnRef "2"), "m_lf")) ::
+  ("2", (#0, "global")) ::
+  ("y", (# (VOwnRef "1"), "l_lf")) ::
+  ("1", (#1, "global")) ::
+  ("x", (#1, "l_lf"))
+  :: nil
+  ).
+
+Example we1_step2_2 : we1_2_1 --> we1_2_2 | "l_lf".
+Proof.
+  apply R_BlockA.
+  apply R_BlockA.
+  apply R_Sub_Seq.
+  apply R_Declare with (lx := "z"). auto.
+Qed.
+
+Definition we1_3 : (term * store) :=
+  (
+  TBlock (
+      (TBlock (
+      TSeq
+        (TAssignment (LVar "y") (TBorrow (LVar "z")))
+        (
+        TSeq
+          (TAssignment (LVar "y") (TMove (LVar "z")))
+          (
+          TSeq
+            (TMove (LDeref (LVar "y")))
+            (TValue VUnit)
+          )
+        )
+      ) "m_lf")
+  ) "l_lf"
+  ,
+  ("z", (# (VOwnRef "2"), "m_lf")) ::
+  ("2", (#0, "global")) ::
+  ("y", (# (VOwnRef "1"), "l_lf")) ::
+  ("1", (#1, "global")) ::
+  ("x", (#1, "l_lf"))
+  :: nil
+  ).
+
+Example we1_step2_3 : we1_2_2 --> we1_3 | "l_lf".
+Proof.
+  apply R_BlockA.
+  apply R_BlockA.
+  apply R_Seq.
+  apply D_cons_other.
+  intros l H; discriminate.
+Qed.
+
+Example we1_step2 : we1_2 -->* we1_3 | "l_lf".
+Proof.
+  apply multi_step with (ts2 := we1_2_1); try (apply we1_step2_1).
+  apply multi_step with (ts2 := we1_2_2); try (apply we1_step2_2).
+  apply multi_step with (ts2 := we1_3); try (apply we1_step2_3).
+  apply multi_refl.
+Qed.
+
+Definition we1_3_1 : (term * store) :=
+  (
+  TBlock (
+      (TBlock (
+      TSeq
+        (TAssignment (LVar "y") (TValue (VBorrowRef "z")))
+        (
+        TSeq
+          (TAssignment (LVar "y") (TMove (LVar "z")))
+          (
+          TSeq
+            (TMove (LDeref (LVar "y")))
+            (TValue VUnit)
+          )
+        )
+      ) "m_lf")
+  ) "l_lf"
+  ,
+  ("z", (# (VOwnRef "2"), "m_lf")) ::
+  ("2", (#0, "global")) ::
+  ("y", (# (VOwnRef "1"), "l_lf")) ::
+  ("1", (#1, "global")) ::
+  ("x", (#1, "l_lf"))
+  :: nil
+  ).
+
+Example we1_step3_1 : we1_3 --> we1_3_1 | "l_lf".
+Proof.
+  apply R_BlockA.
+  apply R_BlockA.
+  apply R_Sub_Seq.
+  apply R_Sub_Asg.
+  apply R_Borrow.
+  loc_var.
+Qed.
+
+Definition we1_3_2 : (term * store) :=
+  (
+  TBlock (
+      (TBlock (
+      TSeq
+        (TValue VUnit)
+        (
+        TSeq
+          (TAssignment (LVar "y") (TMove (LVar "z")))
+          (
+          TSeq
+            (TMove (LDeref (LVar "y")))
+            (TValue VUnit)
+          )
+        )
+      ) "m_lf")
+  ) "l_lf"
+  ,
+  ("z", (# (VOwnRef "2"), "m_lf")) ::
+  ("2", (#0, "global")) ::
+  ("y", (# (VBorrowRef "z"), "l_lf")) ::
+  ("1", (#1, "global")) ::
+  ("x", (#1, "l_lf"))
+  :: nil
+  ).
+
+Example we1_step3_2 : we1_3_1 --> we1_3_2 | "l_lf".
+Proof.
+  apply R_BlockA.
+  apply R_BlockA.
+  apply R_Sub_Seq.
+  apply R_Assign with (st2 := 
+  ("z", (# (VOwnRef "2"), "m_lf")) ::
+  ("2", (#0, "global")) ::
+  ("y", (# (VBorrowRef "z"), "l_lf")) ::
+  ("x", (#1, "l_lf"))
+  :: nil) (pv1 := (# (VOwnRef "1"), "l_lf")).
+  - apply Read with (l := "y").
+    + auto.
+    + loc_var.
+  - simpl. apply D_cons_own with (st3 :=
+  ("z", (# (VOwnRef "2"), "m_lf")) ::
+  ("2", (#0, "global")) ::
+  ("y", (# (VBorrowRef "z"), "l_lf")) ::
+  ("x", (#1, "l_lf"))
+  :: nil
+  ) (l_own := "1").
+    + simpl. reflexivity.
+    + simpl. reflexivity.
+.
+  loc_var.
+Qed.
+
+Definition we1_4 : (term * store) :=
+  (
+  TBlock (
+      (TBlock (
+      TSeq
+        (TAssignment (LVar "y") (TMove (LVar "z")))
+        (
+        TSeq
+          (TMove (LDeref (LVar "y")))
+          (TValue VUnit)
+        )
+      ) "m_lf")
+  ) "l_lf"
+  ,
+  ("z", (# (VOwnRef "2"), "m_lf")) ::
+  ("2", (#0, "global")) ::
+  ("y", (# (VBorrowRef "z"), "l_lf")) ::
+  ("1", (#1, "global")) ::
+  ("x", (#1, "l_lf"))
+  :: nil
+  ).
